src/proof/controllers/common.v
@@ -181,7 +181,7 @@ Definition owner_ref_key (owner_kind : go_string) (owner_meta : ObjectMetaV.t) :
 |}.
 
 Lemma wp_FilterPodsByOwner γ l owner owner_kind meta dq1
-    living_pods pod_dqs children_dq children_keys phase :
+    living_pods pod_dqs children_dq children_keys has_terminating_children :
   {{{ is_pkg_init code.controllers.common.pkg_id.common ∗
       "#Hisk" ∷ is_kubernetes γ l ∗
       "#Hglobal_l" ∷ (global_addr apimodel.ModelState) ↦□ l ∗
@@ -195,7 +195,7 @@ Lemma wp_FilterPodsByOwner γ l owner owner_kind meta dq1
           meta.(ObjectMetaV.UID') children_dq children_keys ∗
       "Hown_terminating_children_frag" ∷
         own_terminating_children_frag γ (owner_ref_key owner_kind meta)
-          meta.(ObjectMetaV.UID') phase ∗
+          meta.(ObjectMetaV.UID') has_terminating_children ∗
       "%Hnodup" ∷ ⌜ NoDup (PodV.key <$> living_pods) ⌝ ∗
       "%Hdom_eq" ∷ ⌜ list_to_set (PodV.key <$> living_pods) =
         filter (λ key, key.(KKey.Kind') = "Pod"%go) children_keys ⌝ ∗
@@ -210,7 +210,7 @@ Lemma wp_FilterPodsByOwner γ l owner owner_kind meta dq1
       ([∗ list] ptr;pod ∈ ptrs;all_pods, PodV.deepown_l ptr pod dq') ∗
       ⌜ ObjectMetaV.without_resource_version <$> (PodV.ObjectMeta' <$> filter is_pod_alive all_pods) ≡ₚ
         ObjectMetaV.without_resource_version <$> (PodV.ObjectMeta' <$> living_pods) ⌝ ∗
-      ⌜ phase = terminating_children.No →
+      ⌜ has_terminating_children = terminating_children.No →
         ObjectMetaV.without_resource_version <$> (PodV.ObjectMeta' <$> all_pods) ≡ₚ
           ObjectMetaV.without_resource_version <$> (PodV.ObjectMeta' <$> living_pods) ⌝ ∗
       ⌜ Forall PodV.valid all_pods ⌝ ∗
@@ -225,7 +225,7 @@ Lemma wp_FilterPodsByOwner γ l owner owner_kind meta dq1
       own_children_frag γ (owner_ref_key owner_kind meta)
         meta.(ObjectMetaV.UID') children_dq children_keys ∗
       own_terminating_children_frag γ (owner_ref_key owner_kind meta)
-        meta.(ObjectMetaV.UID') phase
+        meta.(ObjectMetaV.UID') has_terminating_children
   }}}.
 Proof.
   wp_start as "H". iNamed "H". subst. wp_auto.
@@ -243,7 +243,7 @@ Proof.
   iIntros (index_key) "->". wp_auto.
   iNamedPrefix "Hdeepown_meta" "Htemp_".
   wp_apply (wp_State__ByIndex_podController_combined
-    _ _ _ _ pod_dqs _ _ _ children_dq phase
+    _ _ _ _ pod_dqs _ _ _ children_dq has_terminating_children
     with "[$Hown_pod_meta_frags $Hown_children_frag
       $Hown_terminating_children_frag]").
   { iFrame "#". iFrame "%". iPureIntro. rewrite Htemp_Hdeepown_namespace. rewrite Htemp_Hdeepown_name.
@@ -323,7 +323,7 @@ Proof.
 Qed.
 
 Lemma wp_FilterPodsByOwner_with_spec γ l owner owner_kind meta dq1
-    living_pods pod_dqs children_dq children_keys phase :
+    living_pods pod_dqs children_dq children_keys has_terminating_children :
   {{{ is_pkg_init code.controllers.common.pkg_id.common ∗
       "#Hisk" ∷ is_kubernetes γ l ∗
       "#Hglobal_l" ∷ (global_addr apimodel.ModelState) ↦□ l ∗
@@ -340,7 +340,7 @@ Lemma wp_FilterPodsByOwner_with_spec γ l owner owner_kind meta dq1
           meta.(ObjectMetaV.UID') children_dq children_keys ∗
       "Hown_terminating_children_frag" ∷
         own_terminating_children_frag γ (owner_ref_key owner_kind meta)
-          meta.(ObjectMetaV.UID') phase ∗
+          meta.(ObjectMetaV.UID') has_terminating_children ∗
       "%Hnodup" ∷ ⌜ NoDup (PodV.key <$> living_pods) ⌝ ∗
       "%Hdom_eq" ∷ ⌜ list_to_set (PodV.key <$> living_pods) =
         filter (λ key, key.(KKey.Kind') = "Pod"%go) children_keys ⌝ ∗
@@ -356,7 +356,7 @@ Lemma wp_FilterPodsByOwner_with_spec γ l owner owner_kind meta dq1
         PodV.deepown_l ptr pod dq') ∗
       ⌜ pod_storage_view <$> filter is_pod_alive pods' ≡ₚ
         pod_storage_view <$> living_pods ⌝ ∗
-      ⌜ phase = terminating_children.No →
+      ⌜ has_terminating_children = terminating_children.No →
         pod_storage_view <$> pods' ≡ₚ pod_storage_view <$> living_pods ⌝ ∗
       ⌜ Forall PodV.valid pods' ⌝ ∗
       ⌜ Forall (λ pod,
@@ -377,7 +377,7 @@ Lemma wp_FilterPodsByOwner_with_spec γ l owner owner_kind meta dq1
       own_children_frag γ (owner_ref_key owner_kind meta)
         meta.(ObjectMetaV.UID') children_dq children_keys ∗
       own_terminating_children_frag γ (owner_ref_key owner_kind meta)
-        meta.(ObjectMetaV.UID') phase
+        meta.(ObjectMetaV.UID') has_terminating_children
   }}}.
 Proof.
   wp_start as "H". iNamed "H". subst. wp_auto.
@@ -516,7 +516,7 @@ Proof.
 Qed.
 
 Lemma wp_FilterPodsByOwner_uniform_with_spec γ l owner owner_kind meta dq1
-    living_pods pod_dq children_dq children_keys phase :
+    living_pods pod_dq children_dq children_keys has_terminating_children :
   {{{ is_pkg_init code.controllers.common.pkg_id.common ∗
       "#Hisk" ∷ is_kubernetes γ l ∗
       "#Hglobal_l" ∷ (global_addr apimodel.ModelState) ↦□ l ∗
@@ -533,7 +533,7 @@ Lemma wp_FilterPodsByOwner_uniform_with_spec γ l owner owner_kind meta dq1
           meta.(ObjectMetaV.UID') children_dq children_keys ∗
       "Hown_terminating_children_frag" ∷
         own_terminating_children_frag γ (owner_ref_key owner_kind meta)
-          meta.(ObjectMetaV.UID') phase ∗
+          meta.(ObjectMetaV.UID') has_terminating_children ∗
       "%Hnodup" ∷ ⌜ NoDup (PodV.key <$> living_pods) ⌝ ∗
       "%Hdom_eq" ∷ ⌜ list_to_set (PodV.key <$> living_pods) =
         filter (λ key, key.(KKey.Kind') = "Pod"%go) children_keys ⌝ ∗
@@ -549,7 +549,7 @@ Lemma wp_FilterPodsByOwner_uniform_with_spec γ l owner owner_kind meta dq1
         PodV.deepown_l ptr pod dq') ∗
       ⌜ pod_storage_view <$> filter is_pod_alive pods' ≡ₚ
         pod_storage_view <$> living_pods ⌝ ∗
-      ⌜ phase = terminating_children.No →
+      ⌜ has_terminating_children = terminating_children.No →
         pod_storage_view <$> pods' ≡ₚ pod_storage_view <$> living_pods ⌝ ∗
       ⌜ Forall PodV.valid pods' ⌝ ∗
       ⌜ Forall (λ pod,
@@ -570,7 +570,7 @@ Lemma wp_FilterPodsByOwner_uniform_with_spec γ l owner owner_kind meta dq1
       own_children_frag γ (owner_ref_key owner_kind meta)
         meta.(ObjectMetaV.UID') children_dq children_keys ∗
       own_terminating_children_frag γ (owner_ref_key owner_kind meta)
-        meta.(ObjectMetaV.UID') phase
+        meta.(ObjectMetaV.UID') has_terminating_children
   }}}.
 Proof.
   iIntros (Φ) "H HΦ".
@@ -591,7 +591,7 @@ Proof.
   { subst pod_dqs. rewrite big_sepL2_replicate_r; [done|].
     iExact "Hown_pod_frags". }
   iApply (wp_FilterPodsByOwner_with_spec γ l owner owner_kind meta dq1
-    living_pods pod_dqs children_dq children_keys phase with "[-HΦ]").
+    living_pods pod_dqs children_dq children_keys has_terminating_children with "[-HΦ]").
   { iFrame "#". iFrame "%". iFrame. }
   iNext. iIntros (sl ptrs pods' dq') "H".
   iDestruct "H" as
@@ -717,7 +717,7 @@ Proof.
 Qed.
 
 Lemma wp_FilterPodsByOwner_uniform_combined γ l owner owner_kind meta dq1 dq2
-    living_pods children_keys phase :
+    living_pods children_keys has_terminating_children :
   {{{ is_pkg_init code.controllers.common.pkg_id.common ∗
       "#Hisk" ∷ is_kubernetes γ l ∗
       "#Hglobal_l" ∷ (global_addr apimodel.ModelState) ↦□ l ∗
@@ -729,7 +729,7 @@ Lemma wp_FilterPodsByOwner_uniform_combined γ l owner owner_kind meta dq1 dq2
         meta.(ObjectMetaV.UID') dq2 children_keys ∗
       "Hown_terminating_children_frag" ∷
         own_terminating_children_frag γ (owner_ref_key owner_kind meta)
-          meta.(ObjectMetaV.UID') phase ∗
+          meta.(ObjectMetaV.UID') has_terminating_children ∗
       "%Hnodup" ∷ ⌜ NoDup (PodV.key <$> living_pods) ⌝ ∗
       "%Hdom_eq" ∷ ⌜ list_to_set (PodV.key <$> living_pods) =
         filter (λ key, key.(KKey.Kind') = "Pod"%go) children_keys ⌝ ∗
@@ -755,7 +755,7 @@ Lemma wp_FilterPodsByOwner_uniform_combined γ l owner owner_kind meta dq1 dq2
       own_children_frag γ (owner_ref_key owner_kind meta)
         meta.(ObjectMetaV.UID') dq2 children_keys ∗
       own_terminating_children_frag γ (owner_ref_key owner_kind meta)
-        meta.(ObjectMetaV.UID') phase
+        meta.(ObjectMetaV.UID') has_terminating_children
   }}}.
 Proof.
   iIntros (Φ) "H HΦ".
@@ -771,7 +771,7 @@ Proof.
   { subst pod_dqs. rewrite big_sepL2_replicate_r; [done|].
     iExact "Hown_pod_meta_frags". }
   iApply (wp_FilterPodsByOwner γ l owner owner_kind meta dq1
-    living_pods pod_dqs dq2 children_keys phase with "[-HΦ]").
+    living_pods pod_dqs dq2 children_keys has_terminating_children with "[-HΦ]").
   { iFrame "#". iFrame "%". iFrame. }
   iNext.
   iIntros (sl ptrs all_pods dq') "H".
